LeanFixpoint/VCG/While/Semantics.lean
@@ -1,59 +1,38 @@
 import LeanFixpoint.VCG.While.Types
 
-open Lean
-
-/-! ## Expression Evaluation -/
-
-def AExpr.eval (s : State) : AExpr → Int
-  | .var x     => s x
-  | .lit n     => n
-  | .add a₁ a₂ => a₁.eval s + a₂.eval s
-  | .sub a₁ a₂ => a₁.eval s - a₂.eval s
-  | .mul a₁ a₂ => a₁.eval s * a₂.eval s
-
-def BExpr.eval (s : State) : BExpr → Bool
-  | .tt        => true
-  | .ff        => false
-  | .eq a₁ a₂  => decide (a₁.eval s = a₂.eval s)
-  | .le a₁ a₂  => decide (a₁.eval s ≤ a₂.eval s)
-  | .lt a₁ a₂  => decide (a₁.eval s < a₂.eval s)
-  | .not b     => !b.eval s
-  | .and b₁ b₂ => b₁.eval s && b₂.eval s
-  | .or b₁ b₂  => b₁.eval s || b₂.eval s
-
 /-! ## Big-Step Operational Semantics -/
 
 inductive Ceval : Cmd → State → State → Prop where
   | skip {s} :
     Ceval .skip s s
 
-  | assign {x a s} :
-    Ceval (.assign x a) s (s[x ↦ a.eval s])
+  | assign {x f s} :
+    Ceval (.assign x f) s (s[x ↦ f s])
 
   | seq {c₁ s₁ s₂ c₂ s₃} :
     Ceval c₁ s₁ s₂ →
     Ceval c₂ s₂ s₃ →
     Ceval (.seq c₁ c₂) s₁ s₃
 
-  | ite_true {c₁ s₁ s₂ b c₂} :
-    b.eval s₁ = true →
+  | ite_true {g s₁ s₂ c₁ c₂} :
+    g s₁ = true →
     Ceval c₁ s₁ s₂ →
-    Ceval (.ite b c₁ c₂) s₁ s₂
+    Ceval (.ite g c₁ c₂) s₁ s₂
 
-  | ite_false {c₂ s₁ s₂ b c₁} :
-    b.eval s₁ = false →
+  | ite_false {g s₁ s₂ c₁ c₂} :
+    g s₁ = false →
     Ceval c₂ s₁ s₂ →
-    Ceval (.ite b c₁ c₂) s₁ s₂
+    Ceval (.ite g c₁ c₂) s₁ s₂
 
-  | while_false {b c s} :
-    b.eval s = false →
-    Ceval (.cwhile b c) s s
+  | while_false {g c s} :
+    g s = false →
+    Ceval (.cwhile g c) s s
 
-  | while_true {c s₁ s₂ b s₃} :
-    b.eval s₁ = true →
+  | while_true {g c s₁ s₂ s₃} :
+    g s₁ = true →
     Ceval c s₁ s₂ →
-    Ceval (.cwhile b c) s₂ s₃ →
-    Ceval (.cwhile b c) s₁ s₃
+    Ceval (.cwhile g c) s₂ s₃ →
+    Ceval (.cwhile g c) s₁ s₃
 
 /-! ## Assertions and Hoare Triples -/
 
